Test/Passes/InstructionSelection/RISCV64/icmp_invalid.mlir
@@ -1,14 +1,13 @@
-// RUN: veir-opt %s -p=isel-riscv64 | filecheck %s
+// RUN: not veir-opt %s -p=isel-riscv64 2>&1 | filecheck %s
 
 "builtin.module"() ({
   "func.func"()  <{function_type = (i32, i32, i64) -> ()}> ({
     ^bb0(%a: i32, %b: i32, %c: i64):
         %r_0 = "llvm.icmp"(%a, %b) <{"predicate" = 0 : i64}> : (i32, i32) -> i1
-        // CHECK:           "llvm.icmp"(%{{.*}}, %{{.*}}) <{"predicate" = 0 : i64}> : (i32, i32) -> i1
         %r_2 = "llvm.icmp"(%a, %b) <{"predicate" = 2 : i64}> : (i32, i32) -> i1
-        // CHECK-NEXT:      "llvm.icmp"(%{{.*}}, %{{.*}}) <{"predicate" = 2 : i64}> : (i32, i32) -> i1
         %r_6 = "llvm.icmp"(%c, %b) <{"predicate" = 6 : i64}> : (i64, i32) -> i1
-        // CHECK-NEXT:      "llvm.icmp"(%{{.*}}, %{{.*}}) <{"predicate" = 6 : i64}> : (i64, i32) -> i1
         "func.return"() : () -> ()
   }) : () -> ()
 }) : () -> ()
+
+// CHECK: Error verifying input program: Expected operands to have the same type
